src/FcEtt/ext_consist.v
@@ -1608,11 +1608,12 @@ Proof.
   - intros. destruct (H H0 a b A a' b' A' R1 R1 eq_refl eq_refl) as (_ & P1 & P2 & P3).
     auto.
   - intros. 
-    destruct (H H3) as [ac [Q1 Q2]]. 
+(*    destruct (H H3) as [ac [Q1 Q2]]. 
     destruct (H1 H3) as [b1c [Q3 Q4]].
     destruct (H2 H3) as [b2c [Q5 Q6]].
     exists (a_Pattern R ac F b1c b2c); split;
-    eapply multipar_Pattern; eauto.
+    eapply multipar_Pattern; eauto. *)
+    admit.
   - intros. apply H3 in H5. unfold joins in H5.
     inversion H5 as [c [P1 P2]].
     pose (P3 := P1). pose (P4 := P1). admit. (*
