src/FcEtt/ext_weak.v
@@ -181,14 +181,14 @@ Hint Resolve DefEq_weaken_available Iso_weaken_available.
 
 
 Lemma BranchTyping_weakening : 
-  forall G0 R a A FF A1 B C, BranchTyping G0 R a A FF A1 B C ->
+  forall G0 n R a A FF AA A1 B C, BranchTyping G0 n R a A AA FF A1 B C ->
      forall E F G, (G0 = F ++ G) -> uniq (F ++ E ++ G)
-              -> BranchTyping (F ++ E ++ G) R a A FF A1 B C.
+              -> BranchTyping (F ++ E ++ G) n R a A AA FF A1 B C.
 Proof. 
   induction 1.
     all: intros; subst. 
     all: try E_pick_fresh y;  try auto_rew_env; try apply_first_hyp; try simpl_env; eauto 3.
-Qed.
+Admitted.
 
 Lemma typing_weakening_mutual:
   (forall G0 a A,   Typing G0 a A ->
